WIP: fixing sim_add_co

Coq/src/SimRelAddCO.v
@@ -12,7 +12,7 @@ From imm Require Import Events Execution
 Require Import AuxRel AuxDef EventStructure BasicStep Step Consistency 
         LblStep CertRf CertGraph EventToAction ImmProperties
         SimRelCont SimRelEventToAction SimRelSubExec
-        SimRel SimRelCert. 
+        SimRel SimRelCert SimRelCertBasicStep. 
 
 Set Implicit Arguments.
 Local Open Scope program_scope.
@@ -114,59 +114,380 @@ Section SimRelAddCO.
   Notation "'thread_cont_st' tid" :=
     (fun st => existT _ (thread_lts tid) st) (at level 10, only parsing).
 
-  Definition sim_add_co ws (w' : eventid) (S S' : ES.t) : Prop :=
+  Definition sim_ws (w' : eventid) (S S' : ES.t) := fun w => 
+    ⟪ wE : SE S w ⟫ /\
+    ⟪ wW : SW S w ⟫ /\  
+    ⟪ wNCF : ~ (Scf S') w w' ⟫ /\
+    ⟪ wE2A : Gco (e2a S' w) (e2a S' w') ⟫.
+
+  Definition sim_add_co (w' : eventid) (S S' : ES.t) : Prop :=
     ⟪ wE' : SE S' w' ⟫ /\
     ⟪ wW' : SW S' w' ⟫ /\  
-    ⟪ wsE : ws ⊆₁ SE S ⟫ /\  
-    ⟪ wsW : ws ⊆₁ SW S ⟫ /\  
-    ⟪ wsNCF : ws ∩₁ Scf S' w' ⊆₁ ∅ ⟫ /\  
-    ⟪ wsE2A : e2a S □₁ ws ⊆₁ fun w => Gco w (e2a S' w') ⟫ /\  
-    ⟪ CO' : Sco S' ≡ Sco S ∪ ESstep.co_delta S S' ws w' ⟫.
+    (* ⟪ wsE : ws ⊆₁ SE S ⟫ /\ *)
+    (* ⟪ wsW : ws ⊆₁ SW S ⟫ /\ *)
+    (* ⟪ wsNCF : ws ∩₁ Scf S' w' ⊆₁ ∅ ⟫ /\ *)
+    (* ⟪ wsE : ws ⊆₁ fun w => Gco (e2a S' w) (e2a S' w') ⟫ /\   *)
+    ⟪ CO' : Sco S' ≡ Sco S ∪ ESstep.co_delta S S' (sim_ws w' S S') w' ⟫.
 
   Section SimRelAddCOProps. 
-  
-    Lemma weaken_sim_add_co ws w' k k' e e' S S' 
+
+    Lemma sim_wsE w' S S' :
+      sim_ws w' S S' ⊆₁ SE S.
+    Proof. unfold sim_ws. basic_solver. Qed.
+
+    Lemma sim_wsW w' S S' :
+      sim_ws w' S S' ⊆₁ SW S.
+    Proof. unfold sim_ws. basic_solver. Qed.
+
+    Lemma sim_ws_nCF w' S S' (WF : ES.Wf S) :
+      sim_ws w' S S' ⊆₁ set_compl (Scf S' w').
+    Proof. 
+      unfold sim_ws. unfolder.
+      red. intros. desc.
+      by apply wNCF, ES.cf_sym. 
+    Qed.
+
+    Lemma sim_ws_same_loc_e2a w' S S' (WFS : ES.Wf S) (WFG : Wf G) :
+      sim_ws w' S S' ⊆₁ same_loc (Glab ∘ (e2a S')) w'.
+    Proof. 
+      unfold sim_ws.
+      intros w Wx. desc.
+      assert 
+        (same_loc (Glab ∘ e2a S') w' w <-> same_loc Glab (e2a S' w') (e2a S' w)) 
+        as HH. 
+      { basic_solver. }
+      apply HH.
+      apply same_loc_sym.
+      edestruct loceq_same_loc as [E2A_CO E2A_SLOC].
+      { apply loceq_co; eauto. }
+      { apply wE2A. }
+      done. 
+    Qed.
+
+    (* Lemma sim_add_co_e2a_loc_ws w' k k' e e' S S'  *)
+    (*       (st st' st'' : thread_st (ES.cont_thread S k)) *)
+    (*       (SRCC : simrel_cert prog S G sc TC f TC' h k st st'')  *)
+    (*       (BSTEP_ : ESBasicStep.t_ (thread_lts (ES.cont_thread S k)) k k' st st' e e' S S')  *)
+    (*       (SACO : sim_add_co w' S S')  *)
+    (*       (CST_REACHABLE : (lbl_step (ES.cont_thread S k))＊ st' st'')  *)
+    (*       (wEE' : (eq e ∪₁ eq_opt e') w') :  *)
+    (*   sim_ws w' S S' ⊆₁ same_loc (Glab ∘ (e2a S')) w'. *)
+    (* Proof.  *)
+    (*   cdes BSTEP_; cdes SACO. *)
+    (*   assert (ESBasicStep.t e e' S S') as BSTEP. *)
+    (*   { econstructor. eauto. } *)
+    (*   assert (ES.Wf S) as WFS. *)
+    (*   { apply SRCC. } *)
+    (*   unfold sim_ws. *)
+    (*   intros w Wx. desc. *)
+    (*   assert  *)
+    (*     (same_loc (Glab ∘ e2a S') w' w <-> same_loc Glab (e2a S' w') (e2a S' w))  *)
+    (*     as HH.  *)
+    (*   { basic_solver. } *)
+    (*   apply HH. *)
+    (*   apply same_loc_sym. *)
+    (*   edestruct loceq_same_loc as [E2A_CO E2A_SLOC]. *)
+    (*   { apply loceq_co; apply SRCC. } *)
+    (*   { apply wE2A. } *)
+    (*   done.  *)
+    (* Qed. *)
+
+    (* Lemma sim_add_co_e2a_loc_co_ws ws w' k k' e e' S S'  *)
+    (*       (st st' st'' : thread_st (ES.cont_thread S k)) *)
+    (*       (SRCC : simrel_cert prog S G sc TC f TC' h k st st'')  *)
+    (*       (BSTEP_ : ESBasicStep.t_ (thread_lts (ES.cont_thread S k)) k k' st st' e e' S S')  *)
+    (*       (SACO : sim_add_co ws w' S S')  *)
+    (*       (CST_REACHABLE : (lbl_step (ES.cont_thread S k))＊ st' st'')  *)
+    (*       (wEE' : (eq e ∪₁ eq_opt e') w') :  *)
+    (*   ESstep.co_ws S S' w' ⊆₁ same_loc (Glab ∘ (e2a S')) w'. *)
+    (* Proof.  *)
+    (*   admit.  *)
+    (* Admitted. *)
+    (*   cdes BSTEP_; cdes SACO. *)
+    (*   assert (ESBasicStep.t e e' S S') as BSTEP. *)
+    (*   { econstructor. eauto. } *)
+    (*   assert (ES.Wf S) as WFS. *)
+    (*   { apply SRCC. } *)
+    (*   intros w Wx. red.  *)
+    (*   arewrite (loc (Glab ∘ e2a S') w = loc (Glab ∘ e2a S) w). *)
+    (*   { unfold loc, compose. *)
+    (*     erewrite basic_step_e2a_eq_dom; eauto.  *)
+    (*     apply Wx. } *)
+    (*   erewrite same_lab_u2v_dom_loc  *)
+    (*     with (lab1 := Glab ∘ e2a S). *)
+    (*   2 : { eapply same_lab_u2v_dom_comm. eapply e2a_lab. apply SRCC. } *)
+    (*   {  *)
+    (*   {  *)
+      
+    (*   assert  *)
+    (*     (same_loc (Glab ∘ e2a S') w' w <-> same_loc Glab (e2a S' w') (e2a S' w))  *)
+    (*     as HH.  *)
+    (*   { basic_solver. } *)
+    (*   apply HH. *)
+    (*   red.  *)
+    (*   red.  *)
+
+    (*   apply same_loc_sym. *)
+      
+    (*   edestruct loceq_same_loc as [E2A_CO E2A_SLOC]. *)
+    (*   { apply loceq_co; apply SRCC. } *)
+    (*   { eapply wsE2A. basic_solver. } *)
+    (*   arewrite (e2a S' w = e2a S w); auto. *)
+    (*   eapply basic_step_e2a_eq_dom; eauto. *)
+    (* Qed. *)
+
+    Lemma weaken_sim_add_co w' k k' e e' S S' 
           (st st' st'' : thread_st (ES.cont_thread S k))
           (SRCC : simrel_cert prog S G sc TC f TC' h k st st'') 
           (BSTEP_ : ESBasicStep.t_ (thread_lts (ES.cont_thread S k)) k k' st st' e e' S S') 
-          (SACO : sim_add_co ws w' S S') 
+          (SACO : sim_add_co w' S S') 
           (CST_REACHABLE : (lbl_step (ES.cont_thread S k))＊ st' st'') 
           (wEE' : (eq e ∪₁ eq_opt e') w') : 
-      ESstep.add_co ws w' S S'.
+      ESstep.add_co (sim_ws w' S S') w' S S'.
     Proof. 
       cdes BSTEP_; cdes SACO.
       assert (ESBasicStep.t e e' S S') as BSTEP.
       { econstructor. eauto. }
       assert (ES.Wf S) as WFS.
       { apply SRCC. }
+      assert (Wf G) as WFG.
+      { apply SRCC. }
       
       constructor; splits; auto.
       unfold ESstep.co_ws.
       rewrite set_minus_inter_set_compl.
       rewrite !set_subset_inter_r. 
-      splits; auto.
+      splits.
+      all : eauto using sim_wsE, sim_wsW, sim_ws_nCF.
       { intros w Wx.
         assert ((restr_rel (SE S') (same_loc (Slab S'))) w' w) as SLOC.
         { eapply same_lab_u2v_dom_same_loc.
           { eapply basic_step_e2a_same_lab_u2v; eauto; apply SRCC. }
           red; splits; auto.
-          { assert 
-              (same_loc (Glab ∘ e2a S') w' w <-> same_loc Glab (e2a S' w') (e2a S' w)) 
-              as HH. 
-            { basic_solver. }
-            apply HH.
-            apply same_loc_sym.
-            edestruct loceq_same_loc as [E2A_CO E2A_SLOC].
-            { apply loceq_co; apply SRCC. }
-            { eapply wsE2A. basic_solver. }
-            arewrite (e2a S' w = e2a S w); auto.
-            eapply basic_step_e2a_eq_dom; eauto. }
-          eapply ESBasicStep.basic_step_acts_set_mon; eauto. }
+          { eapply sim_ws_same_loc_e2a; eauto. }
+          eapply ESBasicStep.basic_step_acts_set_mon; eauto. 
+          eapply sim_wsE; eauto. }
         red in SLOC. desf. }
-      unfold set_compl.
-      intros x Wx CF. 
-      eapply wsNCF. basic_solver.
     Qed.
+
+    Lemma sim_add_co_e2a_ws ws w' k k' e e' S S' 
+          (st st' st'' : thread_st (ES.cont_thread S k))
+          (SRCC : simrel_cert prog S G sc TC f TC' h k st st'') 
+          (BSTEP_ : ESBasicStep.t_ (thread_lts (ES.cont_thread S k)) k k' st st' e e' S S') 
+          (SACO : sim_add_co ws w' S S') :
+      e2a S' □₁ ws ≡₁ e2a S □₁ ws.
+    Proof.   
+      cdes BSTEP_; cdes SACO.
+      assert (ESBasicStep.t e e' S S') as BSTEP.
+      { econstructor. eauto. }
+      assert (ES.Wf S) as WFS.
+      { apply SRCC. }
+      eapply set_collect_eq_dom; eauto.
+      red. ins. eapply basic_step_e2a_eq_dom; eauto.
+    Qed.
+
+    Lemma sim_add_co_e2a_co_ws ws w' k k' e e' S S' 
+          (st st' st'' : thread_st (ES.cont_thread S k))
+          (SRCC : simrel_cert prog S G sc TC f TC' h k st st'') 
+          (BSTEP_ : ESBasicStep.t_ (thread_lts (ES.cont_thread S k)) k k' st st' e e' S S') 
+          (SACO : sim_add_co ws w' S S') :
+      e2a S' □₁ (ESstep.co_ws S S' w' \₁ ws) ≡₁ e2a S □₁ (ESstep.co_ws S S' w' \₁ ws).
+    Proof.   
+      cdes BSTEP_; cdes SACO.
+      assert (ESBasicStep.t e e' S S') as BSTEP.
+      { econstructor. eauto. }
+      assert (ES.Wf S) as WFS.
+      { apply SRCC. }
+      eapply set_collect_eq_dom; eauto.
+      red. ins. eapply basic_step_e2a_eq_dom; eauto.
+      unfold ESstep.co_ws in SX.
+      generalize SX. basic_solver.
+    Qed.
+    
+    Lemma sim_add_co_e2a_co_ws_minus_co ws w' k k' e e' S S' 
+          (st st' st'' : thread_st (ES.cont_thread S k))
+          (SRCC : simrel_cert prog S G sc TC f TC' h k st st'') 
+          (BSTEP_ : ESBasicStep.t_ (thread_lts (ES.cont_thread S k)) k k' st st' e e' S S') 
+          (SACO : sim_add_co ws w' S S') 
+          (CST_REACHABLE : (lbl_step (ES.cont_thread S k))＊ st' st'') 
+          (wEE' : (eq e ∪₁ eq_opt e') w') : 
+      e2a S' □₁ (ESstep.co_ws S S' w' \₁ ws) ⊆₁ fun w => (Gco)^? (e2a S' w') w. 
+    Proof. 
+      cdes BSTEP_; cdes SACO.
+      assert (ESBasicStep.t e e' S S') as BSTEP.
+      { econstructor. eauto. }
+      assert (ES.Wf S) as WFS.
+      { apply SRCC. }
+      assert (Wf G) as WFG.
+      { apply SRCC. }
+      erewrite sim_add_co_e2a_co_ws; eauto.
+      intros a [w [[CO_WS nWS] EQa]]. subst a.
+      destruct 
+        (classic (e2a S' w' = e2a S w)) 
+        as [EQ | nEQ].
+      { basic_solver. }
+      apply r_step.
+      edestruct wf_co_total as [CO | CO]; eauto.
+      { unfold set_inter. splits.
+        { eapply basic_step_e2a_GE; 
+            eauto; try apply SRCC.
+          { admit. }
+          basic_solver. }
+        { unfold is_w. fold (compose Glab (e2a S') w'). 
+          eapply same_lab_u2v_dom_is_w.
+          { apply same_lab_u2v_dom_comm.
+            eapply basic_step_e2a_same_lab_u2v; 
+              eauto; apply SRCC. }
+          basic_solver. }
+        eauto. }
+      { unfold ESstep.co_ws in CO_WS.
+        apply set_minus_inter_set_compl in CO_WS.
+        edestruct CO_WS as [[[wE wW] wLOC] wNCF].
+        unfolder; splits; auto.
+        { eapply e2a_GE; [apply SRCC|]. basic_solver. }
+        { unfold is_w. fold (compose Glab (e2a S) w). 
+          eapply same_lab_u2v_dom_is_w.
+          { apply same_lab_u2v_dom_comm.
+            eapply e2a_lab; apply SRCC. }
+          basic_solver. }
+        arewrite (e2a S w = e2a S' w).
+        { symmetry. eapply basic_step_e2a_eq_dom; eauto. }
+        symmetry. eapply sim_add_co_e2a_loc_co_ws; eauto. }
+      exfalso. eapply nWS.
+      
+      assert ((e2a S □₁ ws) (e2a S w)) as E2AWw.
+      { apply wsE2A. split; auto. 
+        generalize CO_WS. unfold ESstep.co_ws. basic_solver. }
+      unfolder in E2AWw.
+      generalize E2AWw. basic_solver 10.
+        
+      
+      
+
+          eapply basic_step_e2a_GE; 
+            eauto; try apply SRCC. 
+          { admit. }
+          arewrite (e2a S x = e2a S' x).
+          { symmetry. eapply basic_step_e2a_eq_dom; eauto. }
+          eapply ESBasicStep.basic_step_acts_set_mon in Ex; eauto.
+          basic_solver. }
+        { unfold is_w. fold (compose Glab (e2a S') w'). 
+          eapply same_lab_u2v_dom_is_w.
+          
+        unfold set_inter; splits; auto.
+      2 : { 
+      
+      unfold ESstep.co_ws.
+      
+
+
+
+
+    Lemma sim_add_co_e2a_co ws w' k k' e e' S S' 
+          (st st' st'' : thread_st (ES.cont_thread S k))
+          (SRCC : simrel_cert prog S G sc TC f TC' h k st st'') 
+          (BSTEP_ : ESBasicStep.t_ (thread_lts (ES.cont_thread S k)) k k' st st' e e' S S') 
+          (SACO : sim_add_co ws w' S S') 
+          (CST_REACHABLE : (lbl_step (ES.cont_thread S k))＊ st' st'') 
+          (wEE' : (eq e ∪₁ eq_opt e') w') : 
+      e2a S' □ Sco S' ⊆ Gco.
+    Proof.
+      cdes BSTEP_; cdes SACO.
+      assert (ESBasicStep.t e e' S S') as BSTEP.
+      { econstructor. eauto. }
+      assert (ES.Wf S) as WFS.
+      { apply SRCC. }
+      assert (e2a S' □₁ ws ≡₁ e2a S □₁ ws) as E2Aws.
+      { eapply set_collect_eq_dom; eauto.
+        red. ins. eapply basic_step_e2a_eq_dom; eauto. }
+      rewrite CO'.
+      rewrite collect_rel_union.
+      unionL.
+      { eapply simrel_cert_basic_step_e2a_eqr; eauto; apply SRCC. }
+      unfold ESstep.co_delta.
+      rewrite collect_rel_union, 
+              collect_rel_cross,
+              set_collect_eq.
+      rewrite !crE. relsf.
+      rewrite !cross_union_l, !cross_union_r, !seqA.
+      unionL.
+      { red. intros x y [Wx EQy]. subst y.
+        eapply wsE2A. by eapply E2Aws. }
+      { arewrite (e2a S' □₁ dom_rel (Sew S ⨾ ⦗ws⦘) ⊆₁ e2a S □₁ ws).
+        { rewrite seq_eqv_r. unfolder.
+          intros a [x [[y [EW Wy]] EQx]]. subst a.
+          eexists; splits; eauto.
+          etransitivity.
+          { eapply e2a_ew; [apply SRCC|].
+            apply ES.ew_sym in EW; auto.
+            do 2 eexists; splits; eauto. }
+          symmetry. eapply basic_step_e2a_eq_dom; eauto.
+          eapply ES.ewE in EW; auto. 
+          generalize EW. basic_solver. }
+        red. intros x y [Wx EQy]. subst y.
+        by eapply wsE2A. }
+      { arewrite 
+          (e2a S' □₁ dom_rel (Sco S ⨾ Sew S ⨾ ⦗ws⦘) ⊆₁ dom_rel (Gco ⨾ ⦗ e2a S □₁ ws ⦘)).
+        { rewrite seq_eqv_r. unfolder.
+          intros a [x [[y [z [CO [EW Wy]]]] EQx]]. subst a.
+          eexists; splits; eauto.
+          arewrite (e2a S' x = e2a S x).
+          { eapply basic_step_e2a_eq_dom; eauto.
+            eapply ES.coE in CO; auto. 
+            generalize CO. basic_solver. }
+          arewrite (e2a S y = e2a S z).
+          { eapply e2a_ew; [apply SRCC|].
+            apply ES.ew_sym in EW; auto.
+            do 2 eexists; splits; eauto. }
+          eapply e2a_co; [apply SRCC|].
+          generalize CO. basic_solver 10. }
+        unfolder. ins. desf.
+        eapply co_trans; [apply SRCC | |]; eauto. 
+        eapply wsE2A. basic_solver. }
+      
+      
+        red. intros x y [[z Wx] EQy]. subst y.
+
+eapply basic_step_e2a_eq_dom; eauto.
+            eapply ES.coE in CO; auto. 
+            generalize CO. basic_solver. }
+          eapply co_trans; [apply SRCC| | ].
+          { eapply e2a_co; [apply SRCC|].
+            generalize CO. basic_solver 10. }
+          
+          etransitivity.
+          { eapply e2a_ew; [apply SRCC|].
+            apply ES.ew_sym in EW; auto.
+            do 2 eexists; splits; eauto. }
+          symmetry. eapply basic_step_e2a_eq_dom; eauto.
+          eapply ES.ewE in EW; auto. 
+          generalize EW. basic_solver. }
+        red. intros x y [Wx EQy]. subst y.
+        by eapply wsE2A.
+          eapply E2Aws.
+            
+            eexists; splits; eauto.
+            etransitivity. 
+            { eapply e2a_ew; [apply SRCC|].
+              unfolder.
+          2 : { rewrite <- E2Aws. basic_solver 20.
+          { 
+        red. intros x y [Wx EQy]. subst y.
+        
+        eapply wsE2A.
+        
+
+        eapply E2Aws.
+        
+        eapply set_collect_eq_dom; eauto.
+        red. symmetry.
+        eapply basic_step_e2a_eq_dom; eauto. } 
+      
+        unfolder. ins. desf.
+        eapply wsE2A. unfolder. basic_solver 10.
+      unionL.
+      { 
+    
 
   End SimRelAddCOProps. 
 
